Remove r0/mem_start from encoders/ag32

compiler/backend/ag32/proofs/ag32_machine_configScript.sml
@@ -7,62 +7,59 @@ local open asmSemTheory targetSemTheory ag32_targetTheory in end
 
 val _ = new_theory"ag32_machine_config";
 
-val ag32_init_asm_regs_def = Define `
-  ag32_init_asm_regs mem_start k = if k = 0n then mem_start else 0w`
-
 val ag32_init_asm_state_def = Define`
-  ag32_init_asm_state mem md (r0:word32) = <|
+  ag32_init_asm_state mem md = <|
     be := F;
     lr := 0 ;
     failed := F ;
     align := 2 ;
-    pc := r0;
+    pc := 0w;
     mem := mem;
     mem_domain := md ;
-    regs := ag32_init_asm_regs r0
+    regs := K 0w
   |>`;
 
 val ag32_prog_addresses_def = Define`
-  ag32_prog_addresses num_ffis LENGTH_code LENGTH_data r0 =
-    { w | r0 + n2w heap_start_offset <=+ w ∧ w <+ r0 + n2w (heap_start_offset + heap_size) } ∪
-    { w | r0 + n2w (code_start_offset num_ffis) <=+ w ∧
-          w <+ r0 + n2w (code_start_offset num_ffis + LENGTH_code + 4 * LENGTH_data) } `;
+  ag32_prog_addresses num_ffis LENGTH_code LENGTH_data =
+    { w | n2w heap_start_offset <=+ w ∧ w <+ n2w (heap_start_offset + heap_size) } ∪
+    { w | n2w (code_start_offset num_ffis) <=+ w ∧
+          w <+ n2w (code_start_offset num_ffis + LENGTH_code + 4 * LENGTH_data) } `;
 
 val ag32_startup_addresses_def = Define`
-  ag32_startup_addresses r0 =
-      { w | r0 <=+ w ∧ w <+ r0 + n2w startup_code_size } ∪
-      { w | r0 + n2w heap_start_offset <=+ w ∧ w <+ r0 + n2w (heap_start_offset + 4 * 5) }`;
+  ag32_startup_addresses =
+      { w | w <+ n2w startup_code_size } ∪
+      { w | n2w heap_start_offset <=+ w ∧ w <+ n2w (heap_start_offset + 4 * 5) }`;
 
 val ag32_ccache_interfer_def = Define`
-  ag32_ccache_interfer num_ffis r0 (_,_,ms) =
+  ag32_ccache_interfer num_ffis (_,_,ms) =
     ms with <| PC := (ms.R 0w) ;
-               R := (0w =+ r0 + n2w (ffi_jumps_offset + num_ffis * ffi_offset + 4)) ms.R |>`;
+               R := (0w =+ n2w (ffi_jumps_offset + num_ffis * ffi_offset + 4)) ms.R |>`;
 
 val ag32_ffi_write_mem_update_def = Define`
-  ag32_ffi_write_mem_update name r0 conf bytes new_bytes mem =
+  ag32_ffi_write_mem_update name conf bytes new_bytes mem =
     if (name = "write") then
       if (HD new_bytes = 0w) then
         case bytes of (n1 :: n0 :: off1 :: off0 :: tll) =>
           let k = MIN (w22n [n1; n0]) output_buffer_size in
           let written = TAKE k (DROP (w22n [off1; off0]) tll) in
-            asm_write_bytearray (r0 + n2w output_offset) (conf ++ [0w;0w;n1;n0] ++ written) mem
-      else ((r0 + n2w output_offset) =+ 1w) mem
+            asm_write_bytearray (n2w output_offset) (conf ++ [0w;0w;n1;n0] ++ written) mem
+      else ((n2w output_offset) =+ 1w) mem
     else mem`;
 
 val ag32_ffi_interfer_def = Define`
-  ag32_ffi_interfer ffi_names md r0 (index,new_bytes,ms) =
+  ag32_ffi_interfer ffi_names md (index,new_bytes,ms) =
     let name = EL index ffi_names in
-    let new_mem = ((r0 + n2w (ffi_code_start_offset - 1)) =+ n2w (THE (ALOOKUP FFI_codes name))) ms.MEM in
+    let new_mem = ((n2w (ffi_code_start_offset - 1)) =+ n2w (THE (ALOOKUP FFI_codes name))) ms.MEM in
     let new_mem = asm_write_bytearray (ms.R 3w) new_bytes new_mem in
     let new_mem =
-      ag32_ffi_write_mem_update name r0
+      ag32_ffi_write_mem_update name
         (THE (read_bytearray (ms.R 1w) (w2n (ms.R 2w)) (λa. if a ∈ md then SOME (ms.MEM a) else NONE)))
         (THE (read_bytearray (ms.R 3w) (w2n (ms.R 4w)) (λa. if a ∈ md then SOME (ms.MEM a) else NONE)))
         new_bytes new_mem in
     let exitpc = THE (ALOOKUP ffi_exitpcs name) in
         ms with
           <| PC := (ms.R 0w) ;
-             R := ((0w =+ r0 + n2w exitpc)
+             R := ((0w =+ n2w exitpc)
                    ((1w =+ 0w)
                    ((2w =+ 0w)
                    ((3w =+ 0w)
@@ -77,9 +74,9 @@ val ag32_ffi_interfer_def = Define`
              MEM := new_mem |>`;
 
 val ag32_machine_config_def = Define`
-  ag32_machine_config ffi_names LENGTH_code LENGTH_data r0 =
+  ag32_machine_config ffi_names LENGTH_code LENGTH_data =
   let num_ffis = LENGTH ffi_names in
-  let md = ag32_prog_addresses num_ffis LENGTH_code LENGTH_data r0 in
+  let md = ag32_prog_addresses num_ffis LENGTH_code LENGTH_data in
   <|
     target := ag32_target;
     ptr_reg := 1;
@@ -88,31 +85,29 @@ val ag32_machine_config_def = Define`
     len2_reg := 4;
     callee_saved_regs := [60; 61; 62];
     ffi_names := ffi_names ;
-    ffi_entry_pcs := REVERSE (GENLIST (λi. r0 + n2w (ffi_jumps_offset + i * ffi_offset)) num_ffis);
-    ccache_pc     := r0 + n2w (ffi_jumps_offset + (num_ffis + 0) * ffi_offset);
-    halt_pc       := r0 + n2w (ffi_jumps_offset + (num_ffis + 1) * ffi_offset);
+    ffi_entry_pcs := REVERSE (GENLIST (λi. n2w (ffi_jumps_offset + i * ffi_offset)) num_ffis);
+    ccache_pc     := n2w (ffi_jumps_offset + (num_ffis + 0) * ffi_offset);
+    halt_pc       := n2w (ffi_jumps_offset + (num_ffis + 1) * ffi_offset);
     prog_addresses := md ;
     next_interfer := K I ;
-    ccache_interfer := K (ag32_ccache_interfer num_ffis r0) ;
-    ffi_interfer := K (ag32_ffi_interfer ffi_names md r0)
+    ccache_interfer := K (ag32_ccache_interfer num_ffis) ;
+    ffi_interfer := K (ag32_ffi_interfer ffi_names md)
   |>`
 
 val is_ag32_machine_config_ag32_machine_config = Q.store_thm("is_ag32_machine_config_ag32_machine_config",
-  `is_ag32_machine_config (ag32_machine_config a b c r0)`, EVAL_TAC);
+  `is_ag32_machine_config (ag32_machine_config a b c)`, EVAL_TAC);
 
 val ag32_ffi_mem_domain_def = Define`
-  ag32_ffi_mem_domain r0 =
-    { w | r0 + n2w startup_code_size <=+ w ∧
-          w <+ r0 + n2w ffi_code_start_offset }`;
+  ag32_ffi_mem_domain =
+    { w | n2w startup_code_size <=+ (w:word32) ∧
+          w <+ n2w ffi_code_start_offset }`;
 
 val ag32_ffi_mem_domain_DISJOINT_prog_addresses = Q.store_thm("ag32_ffi_mem_domain_DISJOINT_prog_addresses",
   `num_ffis ≤ LENGTH FFI_codes ∧
-   w2n (r0:word32) + memory_size < dimword (:32) ∧
    code_start_offset num_ffis + lc + ld ≤ memory_size
    ⇒
-   DISJOINT (ag32_ffi_mem_domain r0) (ag32_prog_addresses num_ffis lc ld r0)`,
+   DISJOINT (ag32_ffi_mem_domain) (ag32_prog_addresses num_ffis lc ld)`,
   EVAL_TAC
-  \\ Cases_on`r0`
   \\ strip_tac
   \\ simp[IN_DISJOINT, PULL_FORALL]
   \\ rpt Cases
